theories/InterleaveLists.v
@@ -1,0 +1,49 @@
+From Coq Require Import
+     List
+     Tactics.
+
+Import ListNotations.
+
+Section defns.
+
+Context {T : Type} (prop_l prop_r : T -> Prop).
+Let L := list T.
+
+Inductive InterleavedList : L -> L -> L -> Prop :=
+| tri_l_nil : forall l,
+    Forall prop_r l ->
+    InterleavedList [] l l
+| tri_r_nil : forall l,
+    Forall prop_l l ->
+    InterleavedList l [] l
+| tri_l_cons : forall a b x l,
+    prop_l x ->
+    InterleavedList a b l ->
+    InterleavedList (x :: a) b (x :: l)
+| tri_r_cons : forall a b x l,
+    prop_r x ->
+    InterleavedList a b l ->
+    InterleavedList a (x :: b) (x :: l).
+
+End defns.
+
+Section tests.
+
+Let P := fun (_:nat) => True.
+
+Example example_interleaved_list_1 : InterleavedList P P [] [] [].
+Proof. constructor; auto. Qed.
+
+Example example_interleaved_list_2 : InterleavedList P P [1; 2] [3; 4] [1; 3; 2; 4].
+Proof. repeat (constructor; auto). Qed.
+
+Example example_interleaved_list_3 : InterleavedList P P [1; 2] [3; 4] [3; 1; 4; 2].
+Proof. repeat (constructor; auto). Qed.
+
+Example example_interleaved_list_4 : InterleavedList P P [1; 2] [3; 4] [4; 1; 3; 2].
+Proof. repeat (constructor; auto). Fail easy. Abort.
+
+Example example_interleaved_list_5 : InterleavedList P P [1; 2] [3; 4] [3; 1; 4; 4; 2].
+Proof. repeat (constructor; auto). Fail easy. Abort.
+
+End tests.
